doc/changelog/04-tactics/11906-micromega-booleans.rst
@@ -1,0 +1,4 @@
+- **Added:**
+  :tacn:`lia` is extended to deal with boolean operators e.g. `andb` or `Z.leb`.
+  (As `lia` gets more powerful, this may break proof scripts relying on `lia` failure.)
+  (`#11906 <https://github.com/coq/coq/pull/11906>`_,  by Frédéric Besson).
